coq/clc/clc_soundness.v
@@ -35,7 +35,7 @@ Proof.
       eapply prop; eauto.
   - inv H1.
     + specialize (IHhas_type1 H _ H6).
-      eapply u_prod; eauto.
+      eapply u_arrow; eauto.
       eapply context_convU.
       eapply conv1i; eauto.
       repeat rewrite <- pure_re; eauto.
@@ -43,14 +43,14 @@ Proof.
     + assert ([A +u Γ |-]).
       eapply u_ok; eauto; repeat rewrite <-pure_re; eauto.
       specialize (IHhas_type2 H1 _ H6).
-      eapply u_prod; eauto.
+      eapply u_arrow; eauto.
   - inv H1.
     + specialize (IHhas_type1 H _ H6).
-      eapply l_prod; eauto.
+      eapply l_arrow; eauto.
     + assert ([□ Γ |-]).
       eapply n_ok; eauto.
       specialize (IHhas_type2 H1 _ H6).
-      eapply l_prod; eauto.
+      eapply l_arrow; eauto.
   - inv H1.
     + specialize (IHhas_type1 H _ H6).
       eapply u_lolli; eauto.
@@ -71,48 +71,113 @@ Proof.
       eapply l_lolli; eauto.
   - inv H1.
   - inv H1.
-  - inv H1.
-    pose proof (pure_re H0).
+  - pose proof (pure_re H0).
+    rewrite H2 in H0_.
     pose proof H0_.
-    rewrite H1 in H0_.
+    inv H1.
     destruct s.
-    + apply u_prod_inv in H0_. first_order.
+    + assert (Arrow A B U ~> Arrow A' B U).
+      constructor; eauto.
+      specialize (IHhas_type1 H _ H1).
+      apply u_arrow_inv in H3; first_order.
+      apply: conversion.
+      apply: conv_sub.
+      apply: conv_sym.
+      apply: conv1; eauto.
+      eauto.
+      apply: arrow_lam; eauto.
+      apply: context_convU.
+      apply: conv_sym.
+      apply: conv1; eauto.
+      eauto.
+      eauto.
+    + assert (Arrow A B L ~> Arrow A' B L).
+      constructor; eauto.
+      specialize (IHhas_type1 H _ H1).
+      apply l_arrow_inv in H3; first_order.
+      apply: conversion.
+      apply: conv_sub.
+      apply: conv_sym.
+      apply: conv1; eauto.
+      eauto.
+      apply: arrow_lam; eauto.
+      apply: context_convL.
+      apply: conv_sym.
+      apply: conv1; eauto.
+      eauto.
+      eauto.
+    destruct s.
+    + apply u_arrow_inv in H0_. first_order.
       assert ([A +u Γ |-]).
       eapply u_ok; eauto.
-      specialize (IHhas_type2 H6 _ H3).
-      eapply prod_lam; eauto.
-    + apply l_prod_inv in H0_. first_order.
+      specialize (IHhas_type2 H5 _ H8).
+      eapply arrow_lam; eauto.
+      rewrite <-pure_re in H3; eauto.
+    + apply l_arrow_inv in H0_. first_order.
       assert ([A +l Γ |-]).
       eapply l_ok; eauto.
-      specialize (IHhas_type2 H6 _ H3).
-      eapply prod_lam; eauto.
-  - inv H1.
-    pose proof H0_.
+      specialize (IHhas_type2 H5 _ H8).
+      eapply arrow_lam; eauto.
+      rewrite <-pure_re in H3; eauto.
+  - pose proof H0_.
+    pose proof (re_ok H).
+    inv H1.
     destruct s.
-    + apply u_lolli_inv in H0_; first_order.
+    + assert (Lolli A B U ~> Lolli A' B U).
+      constructor; eauto.
+      specialize (IHhas_type1 H2 _ H1).
+      apply u_lolli_inv in H0; first_order.
+      apply: conversion.
+      apply: conv_sub.
+      apply: conv_sym.
+      apply: conv1; eauto.
+      eauto.
+      apply: lolli_lam; eauto.
+      apply: context_convU.
+      apply: conv_sym.
+      apply: conv1; eauto.
+      eauto.
+      eauto.
+    + assert (Lolli A B L ~> Lolli A' B L).
+      constructor; eauto.
+      specialize (IHhas_type1 H2 _ H1).
+      apply l_lolli_inv in H0; first_order.
+      apply: conversion.
+      apply: conv_sub.
+      apply: conv_sym.
+      apply: conv1; eauto.
+      eauto.
+      apply: lolli_lam; eauto.
+      apply: context_convL.
+      apply: conv_sym.
+      apply: conv1; eauto.
+      eauto.
+      eauto.
+    destruct s.
+    + apply u_lolli_inv in H0_. first_order.
       assert ([A +u Γ |-]).
       eapply u_ok; eauto.
-      specialize (IHhas_type2 H4 _ H2).
+      specialize (IHhas_type2 H4 _ H7).
       eapply lolli_lam; eauto.
-    + apply l_lolli_inv in H0_; first_order.
+    + apply l_lolli_inv in H0_. first_order.
       assert ([A +l Γ |-]).
       eapply l_ok; eauto.
-      specialize (IHhas_type2 H4 _ H2).
+      specialize (IHhas_type2 H4 _ H7).
       eapply lolli_lam; eauto.
   - pose proof (merge_context_ok_inv H1 H). inv H3.
     inv H2.
     + pose proof (validity H4 H0_); first_order.
       eapply substitutionU; eauto.
-      eapply prod_lam_inv in H0_; eauto.
+      eapply arrow_lam_inv in H0_; eauto.
     + specialize (IHhas_type1 H4 _ H8).
-      eapply u_prod_app; eauto.
+      eapply u_arrow_app; eauto.
     + specialize (IHhas_type2 H5 _ H8).
       assert (B.[n'/] === B.[n/]).
       apply conv_beta.
       apply conv1i; eauto.
       apply conv_sub in H2.
       pose proof (validity H4 H0_); first_order.
-      apply u_prod_inv in H3; first_order.
+      apply u_arrow_inv in H3; first_order.
       assert ([%Γ |- B.[n/] :- (Sort x1 x2).[n/] ]).
       eapply substitutionU; eauto.
       pose proof (pure_re H0).
@@ -120,27 +185,27 @@ Proof.
       rewrite H7. rewrite H10. rewrite H11.
       apply merge_re_re_re.
       eapply conversion; eauto.
-      eapply u_prod_app; eauto.
+      eapply u_arrow_app; eauto.
   - pose proof (merge_context_ok_inv H0 H). inv H2.
     inv H1.
     + pose proof (validity H3 H0_); first_order.
       eapply substitutionL; eauto.
-      eapply prod_lam_inv in H0_; eauto.
+      eapply arrow_lam_inv in H0_; eauto.
     + specialize (IHhas_type1 H3 _ H7).
-      eapply l_prod_app; eauto.
+      eapply l_arrow_app; eauto.
     + specialize (IHhas_type2 H4 _ H7).
       assert (B.[n'/] === B.[n/]).
       apply conv_beta.
       apply conv1i; eauto.
       apply conv_sub in H1.
       pose proof (validity H3 H0_); first_order.
-      apply l_prod_inv in H2; first_order.
+      apply l_arrow_inv in H2; first_order.
       assert ([%Γ |- B.[n/] :- (Sort x1 x2).[n/] ]).
       eapply substitutionN; eauto.
       pose proof (merge_re_re H0). inv H6.
       rewrite <-H8; eauto.
       eapply conversion; eauto.
-      eapply l_prod_app; eauto.
+      eapply l_arrow_app; eauto.
   - pose proof (merge_context_ok_inv H1 H). inv H3.
     inv H2.
     + pose proof (validity H4 H0_); first_order.
@@ -201,16 +266,16 @@ Proof.
   apply H0.
 Qed.
 
-Lemma canonical_prod m C :
+Lemma canonical_arrow m C :
   [ nil |- m :- C ] -> value m ->
   forall A B s, 
-    C <: Prod A B s -> exists m', m = Lam m'.
+    C <: Arrow A B s -> exists A' m' s', m = Lam A' m' s'.
 Proof.
   intros.
   dependent induction H; try (exfalso; solve_sub).
   - inv H.
   - inv H.
-  - exists n; eauto.
+  - exists A. exists n. exists s. eauto.
   - eapply IHhas_type2; eauto.
     eapply sub_trans; eauto.
 Qed.
@@ -218,13 +283,13 @@ Qed.
 Lemma canonical_lolli m C :
   [ nil |- m :- C ] -> value m ->
   forall A B s, 
-    C <: Lolli A B s -> exists m', m = Lam m'.
+    C <: Lolli A B s -> exists A' m' s', m = Lam A' m' s'.
 Proof.
   intros.
   dependent induction H; try (exfalso; solve_sub).
   - inv H.
   - inv H.
-  - exists n; eauto.
+  - exists A. exists n. exists s. eauto.
   - eapply IHhas_type2; eauto.
     eapply sub_trans; eauto.
 Qed.
@@ -245,10 +310,10 @@ Proof.
     specialize (IHhas_type1 H2).
     specialize (IHhas_type2 H2).
     destruct IHhas_type1; destruct IHhas_type2.
-    + assert (exists m', m = Lam m').
-      eapply canonical_prod; eauto.
-      destruct H5; subst.
-      exists (x.[n/]).
+    + assert (exists A' m' s', m = Lam A' m' s').
+      eapply canonical_arrow; eauto.
+      first_order; subst.
+      exists (x0.[n/]).
       apply step_beta; eauto.
     + destruct H4.
       exists (App m x).
@@ -265,10 +330,10 @@ Proof.
     specialize (IHhas_type1 H1).
     specialize (IHhas_type2 H1).
     destruct IHhas_type1; destruct IHhas_type2.
-    + assert (exists m', m = Lam m').
-      eapply canonical_prod; eauto.
-      destruct H4; subst.
-      exists (x.[n/]).
+    + assert (exists A' m' s', m = Lam A' m' s').
+      eapply canonical_arrow; eauto.
+      first_order; subst.
+      exists (x0.[n/]).
       apply step_beta; eauto.
     + destruct H3.
       exists (App m x).
@@ -285,10 +350,10 @@ Proof.
     specialize (IHhas_type1 H2).
     specialize (IHhas_type2 H2).
     destruct IHhas_type1; destruct IHhas_type2.
-    + assert (exists m', m = Lam m').
+    + assert (exists A' m' s', m = Lam A' m' s').
       eapply canonical_lolli; eauto.
-      destruct H5; subst.
-      exists (x.[n/]).
+      first_order; subst.
+      exists (x0.[n/]).
       apply step_beta; eauto.
     + destruct H4.
       exists (App m x).
@@ -305,10 +370,10 @@ Proof.
     specialize (IHhas_type1 H1).
     specialize (IHhas_type2 H1).
     destruct IHhas_type1; destruct IHhas_type2.
-    + assert (exists m', m = Lam m').
+    + assert (exists A' m' s', m = Lam A' m' s').
       eapply canonical_lolli; eauto.
-      destruct H4; subst.
-      exists (x.[n/]).
+      first_order; subst.
+      exists (x0.[n/]).
       apply step_beta; eauto.
     + destruct H3.
       exists (App m x).
